src/ecPrinting.ml
@@ -1253,7 +1253,6 @@ let string_of_hcmp = function
 
 let pp_cost_proj fmt (p : cost_proj) =
   match p with
-  | Conc       -> Format.fprintf fmt "conc"
   | Intr  f    -> Format.fprintf fmt "%s:intr" f
   | Param p    -> Format.fprintf fmt "%s:%s.%s" p.proc p.param_m p.param_p
 
